day1/simple.fsti
@@ -50,14 +50,12 @@ val constant    : (#a:Type) -> (#b:Type) -> b -> a -> Tot b
 
 val lookup      : name -> context -> option info
 
-val lengthInfer : term infer -> nat
-val lengthCheck : term check -> nat
+val length      : (#a:Type) -> term a -> nat
 
-val substInfer  : nat -> term infer -> (e:term infer) -> Tot (term infer) (decreases e)
-val substCheck  : nat -> term infer -> (e:term check) -> Tot (term check) (decreases e)
+val subst       : (#a:Type) -> nat -> term infer -> (e:term a) -> Tot (term a) (decreases e)
 
 val kindInfer   : context -> typeL -> kindL -> result unit 
 
-val typeInfer   : nat -> context -> (e:term infer) -> Tot (result typeL) (decreases (lengthInfer e))
-val typeCheck   : nat -> context -> (e:term check) -> (t:typeL) -> Tot (result unit) (decreases %[lengthCheck e;t])
+val typeInfer   : nat -> context -> (e:term infer) -> Tot (result typeL) (decreases (length e))
+val typeCheck   : nat -> context -> (e:term check) -> (t:typeL) -> Tot (result unit) (decreases %[length e;t])
 val typeInfer0  : context -> term infer -> result typeL
